.

LeanYjs/Network/CausalOrder.lean
@@ -6,24 +6,304 @@ abbrev CausalOrder A := PartialOrder A
 
 section CausalOrder
 
+class Operation (A : Type) where
+  State : Type
+  Error : Type
+  effect : A → State → Except Error State
+
 variable {A : Type} [DecidableEq A] (hb : CausalOrder A)
 
 def hb_concurrent (a b : A) : Prop :=
   ¬ (hb.le a b) ∧ ¬ (hb.le b a)
 
-def hb_consistent (list : List A) : Prop :=
-  ∀ a b, a ∈ list → b ∈ list → list.idxOf? a < list.idxOf? b → hb.le a b
+inductive hb_consistent : List A → Prop where
+  | nil : hb_consistent []
+  | cons : ∀ (a : A) (ops : List A),
+      hb_consistent ops →
+      (∀ b, b ∈ ops → ¬ b ≤ a) →
+      hb_consistent (a :: ops)
 
-def concurrent_commutative (list : List A) (f : A → σ → (Except ε) σ) : Prop :=
+theorem option_not_lt_same {x : Option ℕ} :
+  ¬ x < x := by
+  intro h
+  cases x with
+  | none =>
+    simp at h
+  | some n =>
+    simp at h
+
+theorem List.memf_idxOf?_eq_some {a : A} {l : List A} :
+  a ∈ l → ∃ idx, l.idxOf? a = some idx := by
+  induction l with
+  | nil =>
+    simp
+  | cons b l ih =>
+    intro h_mem
+    simp at h_mem
+    cases Decidable.eq_or_ne a b with
+    | inl h_eq =>
+      rw [h_eq]
+      use 0
+      simp [List.idxOf?_cons]
+    | inr h_neq =>
+      have h_mem_tail : a ∈ l := by
+        cases h_mem with
+        | inl => contradiction
+        | inr => assumption
+      specialize ih h_mem_tail
+      obtain ⟨ idx, h_idx ⟩ := ih
+      use idx + 1
+      simp [List.idxOf?_cons, h_idx]
+      intros h_eq
+      subst a
+      contradiction
+
+omit [DecidableEq A] in lemma hb_consistent_tail (a : A) (ops : List A) :
+  (h_consistent : hb_consistent hb (a :: ops)) →
+  hb_consistent hb ops := by
+  intro h_consistent
+  cases h_consistent
+  assumption
+
+omit [DecidableEq A] theorem no_dup_cons_eq (a : A) {ops₀ ops₁ : List A} :
+  (∀ x, x ∈ a :: ops₀ ↔ x ∈ a :: ops₁) →
+  (a :: ops₀).Nodup → (a :: ops₁).Nodup →
+  (∀ x, x ∈ ops₀ ↔ x ∈ ops₁) := by
+  intros h_mem_iff no_dup₀ no_dup₁ x
+  specialize h_mem_iff x
+  simp at h_mem_iff no_dup₀ no_dup₁
+  obtain ⟨ a_not_mem_ops₀, no_dup₀ ⟩ := no_dup₀
+  obtain ⟨ b_not_mem_ops₁, no_dup₁ ⟩ := no_dup₁
+  constructor
+  . intro h_mem_ops₀
+    have h : x = a ∨ x ∈ ops₀ := by
+      right; assumption
+    rw [h_mem_iff] at h
+    cases h with
+    | inl h_eq =>
+      subst h_eq
+      contradiction
+    | inr h_mem_ops₁ =>
+      assumption
+  . intro h_mem_ops₁
+    have h : x = a ∨ x ∈ ops₁ := by
+      right; assumption
+    rw [← h_mem_iff] at h
+    cases h with
+    | inl h_eq =>
+      subst h_eq
+      contradiction
+    | inr h_mem_ops₀ =>
+      assumption
+
+variable [Operation A]
+
+abbrev Effect := Operation.State A → Except (Operation.Error A) (Operation.State A)
+
+def effect (op : A) : Effect (A := A) :=
+  Operation.effect op
+
+def effect_comp (op1 op2 : Effect (A := A)) : Effect (A := A) := fun s => op1 s >>= op2
+
+local infix:99 " ▷ " => effect_comp
+
+theorem effect_comp_assoc (op1 op2 op3 : Effect (A := A)) :
+  effect_comp (effect_comp op1 op2) op3 = effect_comp op1 (effect_comp op2 op3) := by
+  funext s
+  simp [effect_comp]
+  unfold effect_comp
+  simp
+
+def concurrent_commutative (list : List A) : Prop :=
   ∀ a b, a ∈ list → b ∈ list → hb_concurrent hb a b →
-  ∀ s,
-    (f a s >>= f b) = (f b s >>= f a)
+    effect_comp (effect a) (effect b) = effect_comp (effect b) (effect a)
 
-theorem convergent (ops : List A) (init : σ) (f : A → σ → (Except ε) σ)
-  (h_consistent : hb_consistent hb ops)
-  (h_commutative : concurrent_commutative hb ops f) :
-  ∀ permuted_ops,
-    (∀ a, a ∈ ops ↔ a ∈ permuted_ops) →
-    (List.foldlM f init ops) = (List.foldlM f init permuted_ops) :=
+omit [Operation A] in theorem hb_consistent_concurrent (a : A) (ops₀ ops₁ : List A) :
+  hb_consistent hb (ops₀ ++ a :: ops₁) →
+  ∀ x, x ∈ ops₀ → ¬a ≤ x := by
+  intro h_consistent x h_mem
+  induction ops₀ with
+  | nil =>
+    simp at h_mem
+  | cons y ys ih =>
+    simp at h_mem
+    cases h_consistent with
+    | cons b ops h_consistent_tail h_no_lt =>
+      simp at h_no_lt
+      cases h_mem with
+      | inl h_eq =>
+        subst x
+        apply h_no_lt
+        simp
+      | inr h_mem_tail =>
+        apply ih h_consistent_tail h_mem_tail
+
+
+theorem hb_concurrent_foldr {ops₀ ops₁ : List A} :
+  concurrent_commutative hb (ops₀ ++ a :: ops₁) →
+  (∀ x ∈ ops₀, hb_concurrent hb x a) →
+  List.foldr (effect_comp (A := A)) (effect a ▷ init) (List.map (fun a => effect a) ops₀) =
+  effect a ▷ List.foldr (effect_comp (A := A)) init (List.map (fun a => effect a) ops₀) := by
+  induction ops₀ with
+  | nil =>
+    simp
+  | cons b bs ih =>
+    intro h_comm h_concurrent
+    simp
+    rw [ih]
+    . rw [←effect_comp_assoc]
+      have h_effect_b_effect_a_comm : effect b ▷ effect a = effect a ▷ effect b := by
+        apply h_comm
+        . simp
+        . simp
+        . apply h_concurrent; simp
+      rw [h_effect_b_effect_a_comm]
+      rw [effect_comp_assoc]
+    . intros x y h_x_mem h_y_mem
+      apply h_comm
+      . simp at *
+        right; assumption
+      . simp at *
+        right; assumption
+    . intros; apply h_concurrent; simp; right; assumption
+
+theorem hb_consistent_effect_convergent (ops₀ ops₁ : List A) (init : Effect)
+  (h_consistent₀ : hb_consistent hb ops₀)
+  (h_consistent₁ : hb_consistent hb ops₁)
+  (h_commutative : concurrent_commutative hb ops₀)
+  (no_dup₀ : ops₀.Nodup) (no_dup₁ : ops₁.Nodup) :
+  (∀ a, a ∈ ops₀ ↔ a ∈ ops₁) →
+  (ops₀.map (fun a => effect a) |> List.foldr effect_comp init) =
+  (ops₁.map (fun a => effect a) |> List.foldr effect_comp init) :=
+by
+  induction ops₀ generalizing ops₁ init with
+  | nil =>
+    intros h_mem
+    have ops₁_eq_nil : ops₁ = [] := by
+      cases ops₁ with
+      | nil => rfl
+      | cons a ops₁ =>
+        specialize h_mem a
+        simp at h_mem
+    rw [ops₁_eq_nil]
+  | cons a ops₀ ih =>
+    intros h_mem
+    cases ops₁ with
+    | nil =>
+      specialize h_mem a
+      simp at h_mem
+    | cons b ops₁ =>
+      by_cases h_eq : a = b
+      . -- Case a = b
+        simp
+        rw [h_eq]
+        ext s
+        congr 1
+        apply ih
+        . apply hb_consistent_tail hb a ops₀ h_consistent₀
+        . apply hb_consistent_tail hb b ops₁ h_consistent₁
+        . intros a b h_a_mem h_b_mem h_concurrent
+          apply h_commutative
+          . simp; right; assumption
+          . simp; right; assumption
+          . assumption
+        . simp at no_dup₀
+          obtain ⟨ h_no_dup₀ ⟩ := no_dup₀
+          assumption
+        . simp at no_dup₁
+          obtain ⟨ h_no_dup₁ ⟩ := no_dup₁
+          assumption
+        . subst h_eq
+          apply no_dup_cons_eq _ h_mem no_dup₀ no_dup₁
+      . -- Case a ≠ b
+        have ⟨ ops₁_first, ops₁_last, h_ops₁_eq ⟩ : ∃ ops₁_first ops₁_last, ops₁ = ops₁_first ++ a :: ops₁_last := by
+          have h_a_mem_ops₁ : a ∈ ops₁ := by
+            specialize h_mem a
+            simp at h_mem
+            cases h_mem with
+            | inl h_eq' =>
+              subst h_eq'
+              contradiction
+            | inr h_mem' =>
+              assumption
+          rw [List.mem_iff_append] at h_a_mem_ops₁
+          assumption
+        rw [h_ops₁_eq]
+        simp
+        have h_a_concurrent_op₁_first : ∀ x, x ∈ ops₁_first → hb_concurrent hb x a := by
+          intros x h_mem_ops₁_first
+          constructor
+          . cases h_consistent₀ with
+            | cons _ _ h_consistent_tail h_no_lt =>
+              apply h_no_lt
+              have h_x_in_ops1 : x ∈ b :: ops₁ := by
+                rw [h_ops₁_eq]
+                simp
+                right; left; assumption
+              have x_neq_a : x ≠ a := by
+                intro h_eq'
+                rw [h_ops₁_eq] at no_dup₁
+                rw [List.nodup_cons] at no_dup₁
+                simp at no_dup₁
+                obtain ⟨ _, h_no_dup₁ ⟩ := no_dup₁
+                rw [List.nodup_append] at h_no_dup₁
+                obtain ⟨ _, _, h_no_dup_last ⟩ := h_no_dup₁
+                simp at h_no_dup_last
+                apply h_no_dup_last at h_mem_ops₁_first
+                obtain ⟨ h_eq'', _ ⟩ := h_mem_ops₁_first
+                contradiction
+              rw [← h_mem] at h_x_in_ops1
+              simp at h_x_in_ops1
+              cases h_x_in_ops1 with
+              | inl h_eq' =>
+                contradiction
+              | inr h_mem' =>
+                assumption
+          . apply hb_consistent_concurrent hb a (b :: ops₁_first) ops₁_last
+            . rw [h_ops₁_eq] at h_consistent₁
+              assumption
+            . simp; right; assumption
+        . subst h_ops₁_eq
+          have h_concurrent : concurrent_commutative hb (ops₁_first ++ a :: ops₁_last) := by
+            sorry
+          have h_a_b_concurrent : hb_concurrent hb a b := by
+            sorry
+          rw [hb_concurrent_foldr hb h_concurrent h_a_concurrent_op₁_first]
+          rw [<-effect_comp_assoc]
+          rw [h_commutative b a]
+          rw [effect_comp_assoc]
+          congr!
+          rw [ih (b :: ops₁_first ++ ops₁_last) init]
+          simp
+          . cases h_consistent₀
+            assumption
+          . sorry
+          . intros x y h_x_mem h_ey_mem h_concurrent
+            apply h_commutative
+            simp; right; assumption
+            simp; right; assumption
+            assumption
+          . simp at no_dup₀
+            obtain ⟨ ⟩ := no_dup₀
+            assumption
+          . sorry
+          . intros x
+            constructor
+            . intro h_mem₀
+              have h_mem₀_cons : x ∈ a :: ops₀ := by
+                simp; right; assumption
+              rw [h_mem] at h_mem₀_cons
+              simp at *
+              rcases h_mem₀_cons with h_eq' | ⟨ h | ⟨ h | h ⟩ ⟩
+              . left; assumption
+              . right; left; assumption
+              . subst h; obtain ⟨ h_eq'', _ ⟩ := no_dup₀
+                contradiction
+              . right; right; assumption
+            . sorry
+          . rw [h_mem]
+            simp
+          . simp
+          . sorry
 
 end CausalOrder
